Turned [LiveModel] into a self-contained abstraction

fairness/heap_lang/lifting.v
@@ -10,32 +10,32 @@ From trillium.fairness.heap_lang Require Export lang.
 From trillium.fairness.heap_lang Require Import tactics notation.
 Set Default Proof Using "Type".
 
-Canonical Structure ModelO (Mdl : FairModel) := leibnizO Mdl.
-Canonical Structure RoleO (Mdl : FairModel) := leibnizO (Mdl.(fmrole)).
+Canonical Structure ModelO (M : FairModel) := leibnizO M.
+Canonical Structure RoleO (M : FairModel) := leibnizO (M.(fmrole)).
 
-Class heapGpreS Σ (Mdl : FairModel) (LM: LiveModel heap_lang Mdl) := HeapPreG {
+Class heapGpreS Σ `(LM: LiveModel heap_lang M) := HeapPreG {
   heapGpreS_inv :> invGpreS Σ;
   heapGpreS_gen_heap :> gen_heapGpreS loc val Σ;
-  heapGpreS_fairness :> fairnessGpreS Mdl heap_lang LM Σ;
+  heapGpreS_fairness :> fairnessGpreS LM Σ;
 }.
 
-Class heapGS Σ (Mdl: FairModel) LM := HeapG {
-  heap_inG :> heapGpreS Σ Mdl LM;
+Class heapGS Σ `(LM:LiveModel heap_lang M) := HeapG {
+  heap_inG :> heapGpreS Σ LM;
 
   heap_invGS :> invGS Σ;
   heap_gen_heapGS :> gen_heapGS loc val Σ;
 
-  heap_fairnessGS :> fairnessGS Mdl heap_lang LM Σ;
+  heap_fairnessGS :> fairnessGS LM Σ;
 }.
 
-Definition heapΣ (Mdl : FairModel) : gFunctors :=
-  #[ invΣ; gen_heapΣ loc val; fairnessΣ Mdl heap_lang ].
+Definition heapΣ (M : FairModel) : gFunctors :=
+  #[ invΣ; gen_heapΣ loc val; fairnessΣ heap_lang M ].
 
-Global Instance subG_heapPreG {Σ Mdl LM} :
-  subG (heapΣ Mdl) Σ → heapGpreS Σ Mdl LM.
+Global Instance subG_heapPreG {Σ} `{LM : LiveModel heap_lang M} :
+  subG (heapΣ M) Σ → heapGpreS Σ LM.
 Proof. solve_inG. Qed.
 
-#[global] Instance heapG_irisG `{!heapGS Σ Mdl LM} : irisG heap_lang LM Σ := {
+#[global] Instance heapG_irisG `{LM:LiveModel heap_lang M} `{!heapGS Σ LM} : irisG heap_lang LM Σ := {
     state_interp extr auxtr :=
       (⌜valid_state_evolution_fairness extr auxtr⌝ ∗
        gen_heap_interp (trace_last extr).2.(heap) ∗
@@ -45,7 +45,7 @@ Proof. solve_inG. Qed.
 
 Section adequacy.
 
-Lemma posts_of_empty_mapping `{heapGS Σ Mdl} (e1 e: expr) v (tid : nat) (tp : list expr):
+Lemma posts_of_empty_mapping `{heapGS Σ M} (e1 e: expr) v (tid : nat) (tp : list expr):
   tp !! tid = Some e ->
   to_val e = Some v ->
   posts_of tp ((λ (_ : val), 0%nat ↦M ∅) ::  (map (λ '(tnew, e), fork_post (locale_of tnew e)) (prefixes_from [e1] (drop (length [e1]) tp)))) -∗
@@ -126,9 +126,9 @@ Proof.
   - by intros ex atr [[??]?].
 Qed.
 
-Definition rel_always_holds {Σ} `{LM:LiveModel heap_lang Mdl} `{!heapGS Σ Mdl LM}
-           (s:stuckness) (ξ : execution_trace heap_lang → finite_trace Mdl
-                  (option $ fmrole Mdl) → Prop) (c1:cfg heap_lang)
+Definition rel_always_holds {Σ} `{LM:LiveModel heap_lang M} `{!heapGS Σ LM}
+           (s:stuckness) (ξ : execution_trace heap_lang → finite_trace M
+                  (option $ fmrole M) → Prop) (c1:cfg heap_lang)
            (c2:live_model_to_model LM) : iProp Σ :=
   ∀ ex atr c,
     ⌜valid_system_trace ex atr⌝ -∗
@@ -142,19 +142,19 @@ Definition rel_always_holds {Σ} `{LM:LiveModel heap_lang Mdl} `{!heapGS Σ Mdl 
     state_interp ex atr -∗
     |={⊤, ∅}=> ⌜ξ ex (map_underlying_trace atr)⌝.
 
-Theorem strong_simulation_adequacy Σ `{LM:LiveModel heap_lang Mdl}
-    `{!heapGpreS Σ Mdl LM} (s: stuckness) (e1 : expr) σ1 (s1: Mdl) (FR: gset _)
-    (ξ : execution_trace heap_lang → finite_trace Mdl (option $ fmrole Mdl) →
+Theorem strong_simulation_adequacy Σ `(LM:LiveModel heap_lang M)
+    `{!heapGpreS Σ LM} (s: stuckness) (e1 : expr) σ1 (s1: M) (FR: gset _)
+    (ξ : execution_trace heap_lang → finite_trace M (option $ fmrole M) →
          Prop) :
   rel_finitary (sim_rel_with_user LM ξ) →
-  live_roles Mdl s1 ≠ ∅ ->
-  (∀ `{Hinv : !heapGS Σ Mdl LM},
+  live_roles M s1 ≠ ∅ ->
+  (∀ `{Hinv : !heapGS Σ LM},
     ⊢ |={⊤}=>
        (* state_interp (trace_singleton ([e1], σ1)) (trace_singleton (initial_ls (LM := LM) s1 0%nat)) ∗ *)
        ([∗ map] l ↦ v ∈ heap σ1, mapsto l (DfracOwn 1) v) -∗
        frag_model_is s1 -∗
        frag_free_roles_are (FR ∖ live_roles _ s1) -∗
-       has_fuels (Σ := Σ) 0%nat (gset_to_gmap (LM.(lm_fl) s1) (Mdl.(live_roles) s1)) ={⊤}=∗
+       has_fuels (Σ := Σ) 0%nat (gset_to_gmap (LM.(lm_fl) s1) (M.(live_roles) s1)) ={⊤}=∗
        WP e1 @ s; locale_of [] e1; ⊤ {{ v, 0%nat ↦M ∅ }} ∗
        rel_always_holds s ξ ([e1], σ1) (initial_ls (LM := LM) s1 0%nat)) ->
   continued_simulation (sim_rel_with_user LM ξ) (trace_singleton ([e1], σ1)) (trace_singleton (initial_ls (LM := LM) s1 0%nat)).
@@ -193,7 +193,7 @@ Proof.
   (*   - rewrite dom_gset_to_gmap. set_solver. } *)
   iSpecialize ("Hwp" with "Hσ Hmodf Hfr [Hfuelf Hmapf]").
   { rewrite /has_fuels /frag_mapping_is /= map_fmap_singleton. iFrame.
-    iAssert ([∗ set] ρ ∈ live_roles Mdl s1, ρ ↦F (LM.(lm_fl) s1))%I with "[Hfuelf]" as "H".
+    iAssert ([∗ set] ρ ∈ live_roles M s1, ρ ↦F (LM.(lm_fl) s1))%I with "[Hfuelf]" as "H".
     - unfold frag_fuel_is. setoid_rewrite map_fmap_singleton.
       rewrite -big_opS_own //. iApply (own_proper with "Hfuelf").
       rewrite -big_opS_auth_frag. f_equiv. rewrite gset_to_gmap_singletons //.
@@ -204,7 +204,7 @@ Proof.
 
   iModIntro. iFrame "Hwp".
   iSplitL "Hgen Hmoda Hmapa Hfuela HFR".
-  { unfold state_interp. simpl. iFrame. iExists {[ 0%nat := (live_roles Mdl s1) ]}, _.
+  { unfold state_interp. simpl. iFrame. iExists {[ 0%nat := (live_roles M s1) ]}, _.
     iSplitL "Hfuela"; first by rewrite /auth_fuel_is /= fmap_gset_to_gmap //.
     iSplitL "Hmapa"; first by rewrite /auth_mapping_is /= map_fmap_singleton //.
     iSplit; first done.
@@ -236,7 +236,7 @@ Proof.
     pose proof (trace_singleton_starts_in_inv _ _ Hstartatr). simpl.
     simplify_eq.
     iApply (fupd_mask_weaken ∅); first set_solver. iIntros "_ !>".
-    assert (∀ (ρ : fmrole Mdl) (tid : nat),
+    assert (∀ (ρ : fmrole M) (tid : nat),
                ls_mapping (initial_ls (LM := LM) s1 0%nat) !! ρ = Some tid →
                is_Some (([e1], σ1).1 !! tid)) as HA.
     { simpl. intros ρ tid Hsome. apply lookup_gset_to_gmap_Some in Hsome as [??].
@@ -253,8 +253,8 @@ Proof.
       iAssert (0%nat ↦M ∅) with "[Hposts]" as "Hem".
       { rewrite /= Heq /fmap /=. by iDestruct "Hposts" as "[??]". }
       iDestruct "Hsi" as "(_&_&Hsi)".
-      iDestruct "Hsi" as "(%M&%FR'&Hfuela&Hmapa&HFR&%Hinvmap&%Hsmall&Hmodel&HfrFR)".
-      iDestruct (frag_mapping_same 0%nat M with "[Hmapa] Hem") as "%H"; first done.
+      iDestruct "Hsi" as "(%m&%FR'&Hfuela&Hmapa&HFR&%Hinvmap&%Hsmall&Hmodel&HfrFR)".
+      iDestruct (frag_mapping_same 0%nat m with "[Hmapa] Hem") as "%H"; first done.
       iPureIntro. by eapply no_locale_empty.
     + iSplit; iPureIntro.
       { simpl. intros ρ tid Hsome. apply lookup_gset_to_gmap_Some in Hsome as [??].
@@ -275,7 +275,7 @@ Proof.
     apply (trace_singleton_ends_in_inv (L := unit)) in Hendex.
     simpl in *. simplify_eq.
     iDestruct "Hsi" as "((%&%&%Htids)&_&Hsi)".
-    iDestruct "Hsi" as "(%M&%&Hfuela&Hmapa&?&%Hinvmap&%Hsmall&Hmodel&?)".
+    iDestruct "Hsi" as "(%m&%&Hfuela&Hmapa&?&%Hinvmap&%Hsmall&Hmodel&?)".
     iSplit; [|done].
     iSplit; [done|].
     iSplit.
@@ -285,22 +285,22 @@ Proof.
       { destruct (to_val e') as [?|] eqn:Heq; last done.
         iApply posts_of_empty_mapping => //.
         apply from_locale_lookup =>//. }
-      iDestruct (frag_mapping_same tid' M with "Hmapa H") as "%Hlk".
+      iDestruct (frag_mapping_same tid' m with "Hmapa H") as "%Hlk".
       { rewrite /auth_mapping_is. iPureIntro. by eapply no_locale_empty. }
 Qed.
 
-Theorem simulation_adequacy Σ {Mdl: FairModel} {LM} `{!heapGpreS Σ Mdl LM} (s: stuckness) (e1 : expr) σ1 (s1: Mdl) (FR: gset _):
+Theorem simulation_adequacy Σ `(LM:LiveModel heap_lang M) `{!heapGpreS Σ LM} (s: stuckness) (e1 : expr) σ1 (s1: M) (FR: gset _):
   (* The model has finite branching *)
   rel_finitary (sim_rel LM) →
-  live_roles Mdl s1 ≠ ∅ ->
+  live_roles M s1 ≠ ∅ ->
   (* The initial configuration satisfies certain properties *)
   (* A big implication, and we get back a Coq proposition *)
   (* For any proper Aneris resources *)
-  (∀ `{!heapGS Σ Mdl LM},
+  (∀ `{!heapGS Σ LM},
       ⊢ |={⊤}=>
         frag_model_is s1 -∗
         frag_free_roles_are (FR ∖ live_roles _ s1) -∗
-        has_fuels (Σ := Σ) 0%nat (gset_to_gmap (LM.(lm_fl) s1) (Mdl.(live_roles) s1))
+        has_fuels (Σ := Σ) 0%nat (gset_to_gmap (LM.(lm_fl) s1) (M.(live_roles) s1))
         ={⊤}=∗ WP e1 @ s; 0%nat; ⊤ {{ v, 0%nat ↦M ∅ }}
   ) ->
   (* The coinductive pure coq proposition given by adequacy *)
@@ -320,7 +320,7 @@ Proof.
     unfold sim_rel_with_user. intuition. }
 
   rewrite Heq.
-  apply (strong_simulation_adequacy Σ s _ _ _ FR) =>//.
+  apply (strong_simulation_adequacy Σ LM s _ _ _ FR) =>//.
   { rewrite -Heq. done. }
   iIntros (Hinv) "".
   iPoseProof (H Hinv) as ">H". iModIntro. iIntros "Hσ Hm Hfr Hf". iSplitR "".
@@ -328,19 +328,20 @@ Proof.
   - iIntros "!>%%%???????". iApply (fupd_mask_weaken ∅); first set_solver. by iIntros "_ !>".
 Qed.
 
-Theorem simulation_adequacy_inftraces Σ (Mdl : FairModel) `{!heapGpreS Σ Mdl LM} (s: stuckness) FR
-        e1 σ1 (s1: Mdl)
+Theorem simulation_adequacy_inftraces Σ `(LM: LiveModel heap_lang M)
+        `{!heapGpreS Σ LM} (s: stuckness) FR
+        e1 σ1 (s1: M)
         (iex : inf_execution_trace heap_lang)
         (Hvex : valid_inf_exec (trace_singleton ([e1], σ1)) iex)
   :
   (* The model has finite branching *)
   rel_finitary (sim_rel LM)  →
-  live_roles Mdl s1 ≠ ∅ ->
-  (∀ `{!heapGS Σ Mdl LM},
+  live_roles M s1 ≠ ∅ ->
+  (∀ `{!heapGS Σ LM},
       ⊢ |={⊤}=>
      frag_model_is s1 -∗
          frag_free_roles_are (FR ∖ live_roles _ s1) -∗
-         has_fuels (Σ := Σ) 0%nat (gset_to_gmap (LM.(lm_fl) s1) (Mdl.(live_roles) s1))
+         has_fuels (Σ := Σ) 0%nat (gset_to_gmap (LM.(lm_fl) s1) (M.(live_roles) s1))
         ={⊤}=∗ WP e1 @ s; 0%nat; ⊤ {{ v, 0%nat ↦M ∅ }}
   ) ->
   (* The coinductive pure coq proposition given by adequacy *)
@@ -360,26 +361,26 @@ Proof.
   eapply produced_inf_aux_trace_valid_inf.
   Unshelve.
   - econstructor.
-  - apply (simulation_adequacy Σ s _ _ _ FR) => //.
+  - apply (simulation_adequacy Σ LM s _ _ _ FR) => //.
   - done.
 Qed.
 
 Definition heap_lang_extrace : Type := extrace heap_lang.
 
-Theorem simulation_adequacy_traces Σ (Mdl : FairModel) `{!heapGpreS Σ Mdl LM} (s: stuckness) FR
-        e1 (s1: Mdl)
+Theorem simulation_adequacy_traces Σ `(LM : LiveModel heap_lang M) `{!heapGpreS Σ LM} (s: stuckness) FR
+        e1 (s1: M)
         (extr : heap_lang_extrace)
         (Hvex : extrace_valid extr)
         (Hexfirst : (trfirst extr).1 = [e1])
   :
   (* The model has finite branching *)
   rel_finitary (sim_rel LM) →
-  live_roles Mdl s1 ≠ ∅ ->
-  (∀ `{!heapGS Σ Mdl LM},
+  live_roles M s1 ≠ ∅ ->
+  (∀ `{!heapGS Σ LM},
       ⊢ |={⊤}=>
         frag_model_is s1 -∗
          frag_free_roles_are (FR ∖ live_roles _ s1) -∗
-         has_fuels (Σ := Σ) 0%nat (gset_to_gmap (LM.(lm_fl) s1) (Mdl.(live_roles) s1))
+         has_fuels (Σ := Σ) 0%nat (gset_to_gmap (LM.(lm_fl) s1) (M.(live_roles) s1))
         ={⊤}=∗ WP e1 @ s; 0%nat; ⊤ {{ v, 0%nat ↦M ∅ }}
   ) ->
   (* The coinductive pure coq proposition given by adequacy *)
@@ -397,7 +398,7 @@ Proof.
         (trace_singleton (initial_ls (LM := LM) s1 0%nat))
         (from_trace extr)
         iatr.
-  { apply (simulation_adequacy_inftraces Σ Mdl s FR); eauto.
+  { apply (simulation_adequacy_inftraces _ _ s FR); eauto.
     eapply from_trace_preserves_validity; eauto; first econstructor.
     simpl. destruct (trfirst extr) eqn:Heq.
     simpl in Hexfirst. rewrite -Hexfirst Heq //. }
@@ -410,20 +411,21 @@ Proof.
   - apply to_trace_spec.
 Qed.
 
-Theorem simulation_adequacy_model_trace Σ (Mdl : FairModel) `{!heapGpreS Σ Mdl LM} (s: stuckness) FR
-        e1 (s1: Mdl)
+Theorem simulation_adequacy_model_trace Σ `(LM : LiveModel heap_lang M)
+        `{!heapGpreS Σ LM} (s: stuckness) FR
+        e1 (s1: M)
         (extr : heap_lang_extrace)
         (Hvex : extrace_valid extr)
         (Hexfirst : (trfirst extr).1 = [e1])
   :
   (* The model has finite branching *)
   rel_finitary (sim_rel LM) →
-  live_roles Mdl s1 ≠ ∅ ->
-  (∀ `{!heapGS Σ Mdl LM},
+  live_roles M s1 ≠ ∅ ->
+  (∀ `{!heapGS Σ LM},
       ⊢ |={⊤}=>
         frag_model_is s1 -∗
          frag_free_roles_are (FR ∖ live_roles _ s1) -∗
-         has_fuels (Σ := Σ) 0%nat (gset_to_gmap (LM.(lm_fl) s1) (Mdl.(live_roles) s1))
+         has_fuels (Σ := Σ) 0%nat (gset_to_gmap (LM.(lm_fl) s1) (M.(live_roles) s1))
         ={⊤}=∗ WP e1 @ s; 0%nat; ⊤ {{ v, 0%nat ↦M ∅ }}
   ) ->
   (* The coinductive pure coq proposition given by adequacy *)
@@ -432,14 +434,14 @@ Theorem simulation_adequacy_model_trace Σ (Mdl : FairModel) `{!heapGpreS Σ Mdl
 Proof.
   intros Hfb Hlr Hwp.
   destruct (simulation_adequacy_traces
-              Σ Mdl _ FR e1 s1 extr Hvex Hexfirst Hfb Hlr Hwp) as [auxtr Hmatch].
+              Σ _ _ FR e1 s1 extr Hvex Hexfirst Hfb Hlr Hwp) as [auxtr Hmatch].
   destruct (can_destutter_auxtr extr auxtr) as [mtr Hupto] =>//.
   { intros ?? contra. inversion contra. done. }
   eauto.
 Qed.
 
 Theorem simulation_adequacy_terminate Σ `{LM:LiveModel heap_lang Mdl}
-        `{!heapGpreS Σ Mdl LM} (s: stuckness)
+        `{!heapGpreS Σ LM} (s: stuckness)
         e1 (s1: Mdl) FR
         (extr : heap_lang_extrace)
         (Hexfirst : (trfirst extr).1 = [e1])
@@ -448,7 +450,7 @@ Theorem simulation_adequacy_terminate Σ `{LM:LiveModel heap_lang Mdl}
   (* The model has finite branching *)
   rel_finitary (sim_rel LM) →
   live_roles Mdl s1 ≠ ∅ ->
-  (∀ `{!heapGS Σ Mdl LM},
+  (∀ `{!heapGS Σ LM},
       ⊢ |={⊤}=>
         frag_model_is s1 -∗
          frag_free_roles_are (FR ∖ live_roles _ s1) -∗
@@ -460,7 +462,7 @@ Theorem simulation_adequacy_terminate Σ `{LM:LiveModel heap_lang Mdl}
 Proof.
   intros Hterm Hfb Hlr Hwp Hvex Hfair.
   destruct (simulation_adequacy_model_trace
-              Σ Mdl _ FR e1 s1 extr Hvex Hexfirst Hfb Hlr Hwp) as (auxtr&mtr&Hmatch&Hupto).
+              Σ _ _ FR e1 s1 extr Hvex Hexfirst Hfb Hlr Hwp) as (auxtr&mtr&Hmatch&Hupto).
   destruct (infinite_or_finite extr) as [Hinf|] =>//.
   have Hfairaux := fairness_preserved extr auxtr Hinf Hmatch Hfair.
   have Hvalaux := exaux_preserves_validity extr auxtr Hmatch.
@@ -471,21 +473,21 @@ Proof.
   eapply upto_stutter_finiteness =>//.
 Qed.
 
-Theorem simulation_adequacy_terminate_ftm Σ `{FairTerminatingModel Mdl}
-        `{LM : LiveModel heap_lang Mdl}
-        `{!heapGpreS Σ Mdl LM} (s: stuckness)
-        e1 (s1: Mdl) FR
+Theorem simulation_adequacy_terminate_ftm Σ `{FairTerminatingModel M}
+        `(LM : LiveModel heap_lang M)
+        `{!heapGpreS Σ LM} (s: stuckness)
+        e1 (s1: M) FR
         (extr : heap_lang_extrace)
         (Hexfirst : (trfirst extr).1 = [e1])
   :
   (* The model has finite branching *)
   rel_finitary (sim_rel LM) →
-  live_roles Mdl s1 ≠ ∅ ->
-  (∀ `{!heapGS Σ Mdl LM},
+  live_roles M s1 ≠ ∅ ->
+  (∀ `{!heapGS Σ LM},
       ⊢ |={⊤}=>
         frag_model_is s1 -∗
         frag_free_roles_are (FR ∖ live_roles _ s1) -∗
-        has_fuels (Σ := Σ) 0%nat (gset_to_gmap (LM.(lm_fl) s1) (Mdl.(live_roles) s1))
+        has_fuels (Σ := Σ) 0%nat (gset_to_gmap (LM.(lm_fl) s1) (M.(live_roles) s1))
         ={⊤}=∗ WP e1 @ s; 0%nat; ⊤ {{ v, 0%nat ↦M ∅ }}
   ) ->
   (* The coinductive pure coq proposition given by adequacy *)
@@ -676,8 +678,8 @@ Lemma auth_fuel_is_proper `{heapGS Σ Mdl} (x y : gmap (fmrole Mdl) nat):
 Proof. by intros ->. Qed.
 
 Section lifting.
-Context `{LM:LiveModel heap_lang Mdl}.
-Context `{!heapGS Σ Mdl LM}.
+Context `{LM:LiveModel heap_lang M}.
+Context `{!heapGS Σ LM}.
 Implicit Types P Q : iProp Σ.
 Implicit Types Φ : val → iProp Σ.
 Implicit Types efs : list expr.
@@ -794,10 +796,10 @@ Qed.
 Lemma wp_lift_pure_step_no_fork_take_step s1 s2 tid E E' fs1 fs2 fr1 Φ e1 e2 ρ φ:
   PureExec φ 1 e1 e2 -> φ ->
   valid_new_fuelmap (LM := LM) fs1 fs2 s1 s2 ρ ->
-  live_roles Mdl s2 ∖ live_roles Mdl s1 ⊆ fr1 →
-  Mdl.(fmtrans) s1 (Some ρ) s2 ->
+  live_roles M s2 ∖ live_roles M s1 ⊆ fr1 →
+  M.(fmtrans) s1 (Some ρ) s2 ->
   (|={E}[E']▷=> frag_model_is s1 ∗ has_fuels tid fs1 ∗ frag_free_roles_are fr1 ∗
-                 (frag_model_is s2 -∗ frag_free_roles_are (fr1 ∖ (live_roles Mdl s2 ∖ live_roles Mdl s1))
+                 (frag_model_is s2 -∗ frag_free_roles_are (fr1 ∖ (live_roles M s2 ∖ live_roles M s1))
                   -∗ (has_fuels tid fs2 -∗ WP e2 @ tid; E {{ Φ }})))
   ⊢ WP e1 @ tid; E {{ Φ }}.
 Proof.
@@ -837,9 +839,9 @@ Qed.
 Lemma wp_lift_pure_step_no_fork_singlerole_take_step s1 s2 tid E E' (f1 f2: nat) fr Φ e1 e2 ρ φ:
   PureExec φ 1 e1 e2 -> φ ->
   live_roles _ s2 ⊆ live_roles _ s1 ->
-  (f2 ≤ LM.(lm_fl) s2)%nat -> Mdl.(fmtrans) s1 (Some ρ) s2 ->
+  (f2 ≤ LM.(lm_fl) s2)%nat -> M.(fmtrans) s1 (Some ρ) s2 ->
   (|={E}[E']▷=> frag_model_is s1 ∗ frag_free_roles_are fr ∗ has_fuel tid ρ f1 ∗
-   (frag_model_is s2 -∗ frag_free_roles_are fr -∗ (if decide (ρ ∈ live_roles Mdl s2) then has_fuel tid ρ f2 else tid ↦M ∅) -∗
+   (frag_model_is s2 -∗ frag_free_roles_are fr -∗ (if decide (ρ ∈ live_roles M s2) then has_fuel tid ρ f2 else tid ↦M ∅) -∗
                                WP e2 @ tid; E {{ Φ }}))
   ⊢ WP e1 @ tid; E {{ Φ }}.
 Proof.
@@ -847,20 +849,20 @@ Proof.
   rewrite has_fuel_fuels.
   iIntros "H".
   iApply (wp_lift_pure_step_no_fork_take_step _ _ _ _ _ {[ρ := f1]}
-         (if decide (ρ ∈ live_roles Mdl s2) then {[ρ := f2]} else ∅) fr  with "[H]"); eauto.
+         (if decide (ρ ∈ live_roles M s2) then {[ρ := f2]} else ∅) fr  with "[H]"); eauto.
   - repeat split.
     + intros ?. rewrite decide_True //. rewrite lookup_singleton //=.
     + destruct (decide (ρ ∈ live_roles _ s2)); set_solver.
     + set_solver.
-    + intros ρ' Hdom. destruct (decide (ρ ∈ live_roles Mdl s2)); set_solver.
-    + intros ρ' Hneq Hin. destruct (decide (ρ ∈ live_roles Mdl s2)); set_solver.
-    + destruct (decide (ρ ∈ live_roles Mdl s2)); set_solver.
-    + destruct (decide (ρ ∈ live_roles Mdl s2)); set_solver.
+    + intros ρ' Hdom. destruct (decide (ρ ∈ live_roles M s2)); set_solver.
+    + intros ρ' Hneq Hin. destruct (decide (ρ ∈ live_roles M s2)); set_solver.
+    + destruct (decide (ρ ∈ live_roles M s2)); set_solver.
+    + destruct (decide (ρ ∈ live_roles M s2)); set_solver.
   - set_solver.
   - iMod "H". do 2 iModIntro. iMod "H" as "(Hmod&Hfr&Hfuels&Hkont)". iModIntro.
     iFrame "Hmod Hfr Hfuels". iIntros "Hmod Hfr Hfuels". iApply ("Hkont" with "Hmod [Hfr] [Hfuels]").
-    + replace (fr ∖ (live_roles Mdl s2 ∖ live_roles Mdl s1)) with fr; [done|set_solver].
-    + destruct (decide (ρ ∈ live_roles Mdl s2)).
+    + replace (fr ∖ (live_roles M s2 ∖ live_roles M s1)) with fr; [done|set_solver].
+    + destruct (decide (ρ ∈ live_roles M s2)).
       * rewrite -has_fuel_fuels //.
       * iDestruct "Hfuels" as "[Hf _]". rewrite dom_empty_L //.
 Qed.
@@ -1047,12 +1049,12 @@ Proof.
 Qed.
 
 Lemma wp_store_step_singlerole s tid ρ (f1 f2: nat) fr s1 s2 E l v' v :
-  f2 ≤ LM.(lm_fl) s2 -> fmtrans Mdl s1 (Some ρ) s2 ->
+  f2 ≤ LM.(lm_fl) s2 -> fmtrans M s1 (Some ρ) s2 ->
   live_roles _ s2 ⊆ live_roles _ s1 ->
   {{{ ▷ l ↦ v' ∗ ▷ frag_model_is s1 ∗ ▷ has_fuel tid ρ f1 ∗ ▷ frag_free_roles_are fr }}}
     Store (Val $ LitV $ LitLoc l) (Val v) @ s; tid; E
   {{{ RET LitV LitUnit; l ↦ v ∗ frag_model_is s2 ∗ frag_free_roles_are fr ∗
-      (if decide (ρ ∈ live_roles Mdl s2) then has_fuel tid ρ f2 else tid ↦M ∅ ) }}}.
+      (if decide (ρ ∈ live_roles M s2) then has_fuel tid ρ f2 else tid ↦M ∅ ) }}}.
 Proof.
   iIntros (Hfl Htrans ? Φ) "(>Hl & >Hst & >Hfuel1 & > Hfr) HΦ".
   iApply wp_lift_atomic_head_step_no_fork; auto.
@@ -1065,12 +1067,12 @@ Proof.
   rewrite has_fuel_fuels Hexend.
   iMod (@gen_heap_update with "Hsi Hl") as "[Hsi Hl]".
   iMod (update_step_still_alive _ _ _ _ _ _ _ _ _
-            (if decide (ρ ∈ live_roles Mdl s2) then {[ ρ := f2 ]} else ∅)
+            (if decide (ρ ∈ live_roles M s2) then {[ ρ := f2 ]} else ∅)
             with "Hfuel1 Hst Hmi Hfr") as
         (δ2 ℓ) "([%Hlab %Hvse] & Hfuel & Hst & Hfr & Hmod)"; eauto.
   - set_solver.
-  - destruct (decide (ρ ∈ live_roles Mdl s2)); apply head_locale_step; econstructor =>//.
-  - destruct (decide (ρ ∈ live_roles Mdl s2)).
+  - destruct (decide (ρ ∈ live_roles M s2)); apply head_locale_step; econstructor =>//.
+  - destruct (decide (ρ ∈ live_roles M s2)).
     + split; first by intros _; rewrite lookup_singleton /=; lia.
       split; first set_solver.
       split; first set_solver.
@@ -1082,19 +1084,19 @@ Proof.
     iFrame.
     iSplit; first done.
     iApply "HΦ". iFrame.
-    replace (fr ∖ (live_roles Mdl s2 ∖ live_roles Mdl s1))
+    replace (fr ∖ (live_roles M s2 ∖ live_roles M s1))
       with fr; [iFrame|set_solver].
-    destruct (decide (ρ ∈ live_roles Mdl s2)).
+    destruct (decide (ρ ∈ live_roles M s2)).
     + rewrite has_fuel_fuels //.
     + iDestruct "Hfuel" as "[?_]". rewrite dom_empty_L //.
 Qed.
 
 Lemma wp_cmpxchg_fail_step_singlerole s tid ρ (f1 f2: nat) fr s1 s2 E l q v' v1 v2:
-  v' ≠ v1 → vals_compare_safe v' v1 → f2 ≤ LM.(lm_fl) s2 -> Mdl.(fmtrans) s1 (Some ρ) s2 ->
+  v' ≠ v1 → vals_compare_safe v' v1 → f2 ≤ LM.(lm_fl) s2 -> M.(fmtrans) s1 (Some ρ) s2 ->
   live_roles _ s2 ⊆ live_roles _ s1 ->
   {{{ ▷ l ↦{q} v' ∗ ▷ frag_model_is s1 ∗ ▷ has_fuel tid ρ f1 ∗ ▷ frag_free_roles_are fr }}} CmpXchg (Val $ LitV $ LitLoc l) (Val v1) (Val v2) @ s; tid; E
   {{{ RET PairV v' (LitV $ LitBool false); l ↦{q} v' ∗ frag_model_is s2 ∗ frag_free_roles_are fr ∗
-      (if decide (ρ ∈ live_roles Mdl s2) then has_fuel tid ρ f2 else tid ↦M ∅ ) }}}.
+      (if decide (ρ ∈ live_roles M s2) then has_fuel tid ρ f2 else tid ↦M ∅ ) }}}.
 Proof.
   iIntros (?? Hfl Htrans ? Φ) "(>Hl & >Hst & >Hfuel1 & > Hfr) HΦ". iApply wp_lift_atomic_head_step_no_fork; auto.
   iIntros (extr atr K tp1 tp2 σ1 Hval Hexend Hloc) "(% & Hsi & Hmi) !>".
@@ -1105,12 +1107,12 @@ Proof.
   rewrite bool_decide_false //.
   rewrite has_fuel_fuels Hexend.
   iMod (update_step_still_alive _ _ _ _ _ _ _ _ _
-            (if decide (ρ ∈ live_roles Mdl s2) then {[ ρ := f2 ]} else ∅)
+            (if decide (ρ ∈ live_roles M s2) then {[ ρ := f2 ]} else ∅)
             with "Hfuel1 Hst Hmi Hfr") as
         (δ2 ℓ) "([%Hlab %Hvse] & Hfuel & Hst & Hfr & Hmod)"; eauto.
   - set_solver.
-  - destruct (decide (ρ ∈ live_roles Mdl s2)); apply head_locale_step; econstructor =>//.
-  - destruct (decide (ρ ∈ live_roles Mdl s2)).
+  - destruct (decide (ρ ∈ live_roles M s2)); apply head_locale_step; econstructor =>//.
+  - destruct (decide (ρ ∈ live_roles M s2)).
     + split; first by intros _; rewrite lookup_singleton /=; lia.
       split; first set_solver.
       split; first set_solver.
@@ -1122,15 +1124,15 @@ Proof.
     { iPureIntro. simpl in *. split =>//. }
     iFrame.
     iSplit; first done. iApply "HΦ". iFrame.
-    replace (fr ∖ (live_roles Mdl s2 ∖ live_roles Mdl s1)) with fr; [iFrame|set_solver].
-    destruct (decide (ρ ∈ live_roles Mdl s2)).
+    replace (fr ∖ (live_roles M s2 ∖ live_roles M s1)) with fr; [iFrame|set_solver].
+    destruct (decide (ρ ∈ live_roles M s2)).
     + rewrite has_fuel_fuels //.
     + iDestruct "Hfuel" as "[?_]". rewrite dom_empty_L //.
 Qed.
 
 Lemma wp_cmpxchg_suc_step_singlerole_keep_dead  s tid ρ (f1 f2: nat) fr s1 s2 E l v' v1 v2:
   ρ ∉ live_roles _ s2 →
-  v' = v1 → vals_compare_safe v' v1 → f2 < f1 -> Mdl.(fmtrans) s1 (Some ρ) s2 ->
+  v' = v1 → vals_compare_safe v' v1 → f2 < f1 -> M.(fmtrans) s1 (Some ρ) s2 ->
   live_roles _ s2 ⊆ live_roles _ s1 ->
   {{{ ▷ l ↦ v' ∗ ▷ frag_model_is s1 ∗ ▷ has_fuel tid ρ f1 ∗ ▷ frag_free_roles_are fr }}}
     CmpXchg (Val $ LitV $ LitLoc l) (Val v1) (Val v2) @ s; tid; E
@@ -1159,17 +1161,17 @@ Proof.
     iModIntro; iExists δ2, ℓ. iSplit.
     { iPureIntro. simpl in *. split =>//. }
     iFrame. iSplit; first done. iApply "HΦ". iFrame.
-    replace (fr ∖ (live_roles Mdl s2 ∖ live_roles Mdl s1)) with fr; [iFrame|set_solver].
+    replace (fr ∖ (live_roles M s2 ∖ live_roles M s1)) with fr; [iFrame|set_solver].
     by rewrite has_fuel_fuels.
 Qed.
 
 Lemma wp_cmpxchg_suc_step_singlerole s tid ρ (f1 f2: nat) fr s1 s2 E l v' v1 v2:
-  v' = v1 → vals_compare_safe v' v1 → f2 ≤ LM.(lm_fl) s2 -> Mdl.(fmtrans) s1 (Some ρ) s2 ->
+  v' = v1 → vals_compare_safe v' v1 → f2 ≤ LM.(lm_fl) s2 -> M.(fmtrans) s1 (Some ρ) s2 ->
   live_roles _ s2 ⊆ live_roles _ s1 ->
   {{{ ▷ l ↦ v' ∗ ▷ frag_model_is s1 ∗ ▷ has_fuel tid ρ f1 ∗ ▷ frag_free_roles_are fr }}}
     CmpXchg (Val $ LitV $ LitLoc l) (Val v1) (Val v2) @ s; tid; E
   {{{ RET PairV v' (LitV $ LitBool true); l ↦ v2 ∗ frag_model_is s2 ∗ frag_free_roles_are fr ∗
-      (if decide (ρ ∈ live_roles Mdl s2) then has_fuel tid ρ f2 else tid ↦M ∅ ) }}}.
+      (if decide (ρ ∈ live_roles M s2) then has_fuel tid ρ f2 else tid ↦M ∅ ) }}}.
 Proof.
   iIntros (?? Hfl Htrans ? Φ) "(>Hl & >Hst & >Hfuel1 & >Hfr) HΦ".
   iApply wp_lift_atomic_head_step_no_fork; auto.
@@ -1182,12 +1184,12 @@ Proof.
   iMod (@gen_heap_update with "Hsi Hl") as "[Hsi Hl]".
   rewrite has_fuel_fuels Hexend.
   iMod (update_step_still_alive _ _ _ _ _ _ _ _ _
-            (if decide (ρ ∈ live_roles Mdl s2) then {[ ρ := f2 ]} else ∅)
+            (if decide (ρ ∈ live_roles M s2) then {[ ρ := f2 ]} else ∅)
             with "Hfuel1 Hst Hmi Hfr") as
         (δ2 ℓ) "([%Hlab %Hvse] & Hfuel & Hst & Hfr & Hmod)"; eauto.
   - set_solver.
-  - destruct (decide (ρ ∈ live_roles Mdl s2)); apply head_locale_step; econstructor =>//.
-  - destruct (decide (ρ ∈ live_roles Mdl s2)).
+  - destruct (decide (ρ ∈ live_roles M s2)); apply head_locale_step; econstructor =>//.
+  - destruct (decide (ρ ∈ live_roles M s2)).
     + split; first by intros _; rewrite lookup_singleton /=; lia.
       split; first set_solver.
       split; first set_solver.
@@ -1197,8 +1199,8 @@ Proof.
     iModIntro; iExists δ2, ℓ. iSplit.
     { iPureIntro. simpl in *. split =>//. }
     iFrame. iSplit; first done. iApply "HΦ". iFrame.
-    replace (fr ∖ (live_roles Mdl s2 ∖ live_roles Mdl s1)) with fr; [iFrame|set_solver].
-    destruct (decide (ρ ∈ live_roles Mdl s2)).
+    replace (fr ∖ (live_roles M s2 ∖ live_roles M s1)) with fr; [iFrame|set_solver].
+    destruct (decide (ρ ∈ live_roles M s2)).
     + rewrite has_fuel_fuels //.
     + iDestruct "Hfuel" as "[?_]". rewrite dom_empty_L //.
 Qed.
