fairness/examples/yesno/yesno_adequacy.v
@@ -229,9 +229,9 @@ Theorem yesno_terminates
         (Hexfirst : (trfirst extr).1 = [start #N]):
   (∀ tid, fair_ex tid extr) -> terminating_trace extr.
 Proof.
-  assert (heapGpreS yesnoΣ the_fair_model the_model) as HPreG.
+  assert (heapGpreS yesnoΣ the_model) as HPreG.
   { apply _. }
-  eapply (simulation_adequacy_terminate_ftm (Mdl := the_fair_model) yesnoΣ NotStuck _ (N, true) ∅) =>//.
+  eapply (simulation_adequacy_terminate_ftm yesnoΣ the_model NotStuck _ (N, true) ∅) =>//.
   - eapply valid_state_evolution_finitary_fairness_simple.
     intros ?. simpl. apply (model_finitary s1).
   - destruct N; [lia|destruct N; set_solver].
